Utils.thy
@@ -1,0 +1,21 @@
+(*
+    Author:     Vincent Trélat <vincent.trelat@depinfonancy.net>
+*)
+
+theory Utils
+  imports Main "HOL-Library.Multiset"
+begin
+
+definition subset_mset_rel :: "('a multiset * 'a multiset) set" where
+  "subset_mset_rel \<equiv> {(A,B). A <# B}"
+
+primrec multiset_of :: "'a list \<Rightarrow> 'a multiset" where
+  "multiset_of [] = {#}" |
+  "multiset_of (a # x) = multiset_of x + {# a #}"
+
+
+lemma multiset_of_append [simp]:
+  "multiset_of (xs @ ys) = multiset_of xs + multiset_of ys"
+  by (induct xs arbitrary: ys) (auto simp: add_ac)
+
+end
